src/core-props/bir_update_blockScript.sml
@@ -1,0 +1,564 @@
+open HolKernel Parse boolLib bossLib;
+open bir_program_blocksTheory;
+open stringTheory finite_mapTheory pred_setTheory
+open bir_envTheory listTheory
+open bir_programTheory
+open bir_auxiliaryTheory
+open HolBACoreSimps;
+
+
+(* This theory defines functionality for blocks that update multiple
+   variables "in parallel".
+
+   A single update specification states that a certain variable in the
+   environment should be updated to contain the value of a certain
+   expression. If multiple variables should be updated "in parallel",
+   the problem arises that variables used in later expression have
+   already been updated. update-blocks use temporary variables to
+   store the old value and perform a seemingly "parallel"
+   update. However, the value of potentially used temp vars is
+   changed.
+*)
+
+
+
+val _ = new_theory "bir_update_block";
+
+
+(****************************)
+(* Temporary variable names *)
+(****************************)
+
+val bir_temp_var_name_def = Define `bir_temp_var_name vn = STRCAT "tmp_" vn`;
+val bir_is_temp_var_name_def = Define `bir_is_temp_var_name vn = (TAKE 4 vn = "tmp_")`
+
+val bir_temp_var_def = Define `bir_temp_var use_temp (BVar vn ty) =
+  BVar (if use_temp then (bir_temp_var_name vn) else vn) ty`;
+
+val bir_temp_var_name_11 = store_thm ("bir_temp_var_name_11",
+  ``!vn1 vn2. (bir_temp_var_name vn1 = bir_temp_var_name vn2) <=> (vn1 = vn2)``,
+SIMP_TAC list_ss [bir_temp_var_name_def]);
+
+
+val bir_temp_var_name_irreflexive = store_thm ("bir_temp_var_name_irreflexive",
+  ``!vn. bir_temp_var_name vn <> vn``,
+REPEAT STRIP_TAC >>
+`STRLEN (bir_temp_var_name vn) = STRLEN vn` by ASM_REWRITE_TAC[] >>
+FULL_SIMP_TAC std_ss [stringTheory.STRLEN_CAT, bir_temp_var_name_def,
+  stringTheory.STRLEN_THM]);
+
+
+val bir_is_temp_var_name_ALT_DEF = store_thm ("bir_is_temp_var_name_ALT_DEF",
+  ``!vn. bir_is_temp_var_name vn <=> (?vn'. vn = bir_temp_var_name vn')``,
+
+SIMP_TAC std_ss [bir_is_temp_var_name_def, bir_temp_var_name_def] >>
+GEN_TAC >> EQ_TAC >> REPEAT STRIP_TAC >> ASM_SIMP_TAC list_ss [] >>
+REPEAT (
+  Cases_on `vn` >> FULL_SIMP_TAC list_ss [] >>
+  rename1 `TAKE _ vn = _`
+));
+
+
+val bir_is_temp_var_name_REWR = store_thm ("bir_is_temp_var_name_REWR",
+  ``!vn. bir_is_temp_var_name (bir_temp_var_name vn)``,
+METIS_TAC[bir_is_temp_var_name_ALT_DEF]);
+
+
+val bir_temp_var_REWRS = store_thm ("bir_temp_var_REWRS",
+  ``(!v. bir_temp_var F v = v) /\
+    (!v ut. bir_var_type (bir_temp_var ut v) = bir_var_type v) /\
+    (!v ut. bir_var_name (bir_temp_var ut v) =
+         (if ut then (bir_temp_var_name (bir_var_name v)) else bir_var_name v))``,
+
+REPEAT CONJ_TAC >> Cases >> (
+  SIMP_TAC std_ss [bir_temp_var_def, bir_var_type_def, bir_var_name_def]
+));
+
+
+
+(****************************)
+(* Update descriptions      *)
+(****************************)
+
+val _ = Datatype `bir_updateB_desc_t = BUpdateDescB bir_var_t bir_exp_t bir_val_t bool`;
+
+val bir_updateB_desc_t_11 = DB.fetch "-" "bir_updateB_desc_t_11";
+
+val bir_updateB_desc_var_def =
+  Define `bir_updateB_desc_var (BUpdateDescB var _ _ _) = var`;
+
+val bir_updateB_desc_temp_var_def =
+  Define `bir_updateB_desc_temp_var (BUpdateDescB var _ _ use_temp) =
+          bir_temp_var use_temp var`;
+
+val bir_updateB_desc_exp_def =
+  Define `bir_updateB_desc_exp (BUpdateDescB _ e _ _) = e`;
+
+val bir_updateB_desc_value_def =
+  Define `bir_updateB_desc_value (BUpdateDescB _ _ v _) = v`;
+
+val bir_updateB_desc_use_temp_def =
+  Define `bir_updateB_desc_use_temp (BUpdateDescB _ _ _ ut) = ut`;
+
+
+val bir_updateB_desc_ACCESSORS = save_thm ("bir_updateB_desc_ACCESSORS",
+  LIST_CONJ [bir_updateB_desc_var_def, bir_updateB_desc_temp_var_def,
+             bir_updateB_desc_exp_def, bir_updateB_desc_value_def,
+             bir_updateB_desc_use_temp_def]);
+
+
+
+val bir_updateB_desc_OK_def = Define `
+  bir_updateB_desc_OK env (BUpdateDescB var e v use_temp) <=> (
+     (* Types fit *)
+     (type_of_bir_val v = SOME (bir_var_type var)) /\
+
+     (* The varname is not a temp one *)
+     (~(bir_is_temp_var_name (bir_var_name var))) /\
+
+     (* Variable and if used the temp var are declared *)
+     bir_env_var_is_declared env var /\
+     bir_env_var_is_declared env (bir_temp_var use_temp var) /\
+
+     (* The expression really evaluates to the given value *)
+     (bir_eval_exp e env = v)
+  )`
+
+
+val bir_update_blockB_desc_OK_def = Define `
+  bir_update_blockB_desc_OK env updates <=> (
+
+  (* All descs are well-formed *)
+  EVERY (bir_updateB_desc_OK env) updates /\
+
+  (* A var is only updated once *)
+  (ALL_DISTINCT (MAP (\up. bir_var_name (bir_updateB_desc_var up)) updates)) /\
+
+  (* Previous assigments do not interfer. *)
+  (!i j var. (i < LENGTH updates) /\ (j < i) /\
+             var IN (bir_vars_of_exp (bir_updateB_desc_exp (EL i updates))) ==>
+             (bir_var_name var <>
+                 bir_var_name (bir_updateB_desc_temp_var (EL j updates)))))`;
+
+
+
+val bir_update_blockB_desc_OK_NULL = store_thm("bir_update_blockB_desc_OK_NULL", ``
+  !env. bir_update_blockB_desc_OK env []``,
+SIMP_TAC list_ss [bir_update_blockB_desc_OK_def]);
+
+
+val bir_update_blockB_desc_OK_SNOC = store_thm("bir_update_blockB_desc_OK_SNOC", ``
+  !env updates up.
+  bir_update_blockB_desc_OK env (SNOC up updates) <=>
+
+  (bir_update_blockB_desc_OK env updates /\
+  (EVERY (\up'. ~(bir_var_name (bir_updateB_desc_var up') = bir_var_name (bir_updateB_desc_var up))) updates) /\
+
+  (let used_var_name_set = IMAGE bir_var_name (bir_vars_of_exp (bir_updateB_desc_exp up)) in
+  (EVERY (\up'. ~(bir_var_name (bir_updateB_desc_temp_var up') IN used_var_name_set)) updates)) /\
+  (bir_updateB_desc_OK env up)
+)``,
+
+SIMP_TAC (list_ss++boolSimps.EQUIV_EXTRACT_ss) [bir_update_blockB_desc_OK_def,
+  EVERY_SNOC, MAP_SNOC, prim_recTheory.LESS_THM, ALL_DISTINCT_SNOC, MEM_MAP,
+  RIGHT_AND_OVER_OR, DISJ_IMP_THM, FORALL_AND_THM, EL_LENGTH_SNOC,
+  EL_SNOC, LET_THM, IN_IMAGE, EVERY_MEM, MEM_EL, GSYM LEFT_FORALL_IMP_THM,
+  GSYM RIGHT_FORALL_OR_THM] >>
+METIS_TAC[EL_SNOC]);
+
+
+val bir_update_blockB_desc_OK_CONS = store_thm("bir_update_blockB_desc_OK_CONS", ``
+  !env updates up.
+  bir_update_blockB_desc_OK env (up :: updates) <=>
+
+  (bir_update_blockB_desc_OK env updates /\
+  (EVERY (\up'. ~(bir_var_name (bir_updateB_desc_var up') = bir_var_name (bir_updateB_desc_var up))) updates) /\
+  (bir_updateB_desc_OK env up) /\
+  (EVERY (\up'. ~(bir_var_name (bir_updateB_desc_temp_var up) IN
+      IMAGE bir_var_name (bir_vars_of_exp (bir_updateB_desc_exp up')))) updates)
+)``,
+
+SIMP_TAC (list_ss++boolSimps.EQUIV_EXTRACT_ss) [bir_update_blockB_desc_OK_def,
+  FORALL_AND_THM, EVERY_MEM, MEM_MAP, indexedListsTheory.LT_SUC,
+  RIGHT_AND_OVER_OR, DISJ_IMP_THM, GSYM LEFT_EXISTS_AND_THM, GSYM LEFT_FORALL_IMP_THM,
+  LEFT_AND_OVER_OR, GSYM RIGHT_EXISTS_AND_THM, IN_IMAGE] >>
+REPEAT STRIP_TAC >>
+METIS_TAC[MEM_EL]);
+
+
+
+val bir_update_blockB_desc_OK_VARNAME_UNIQUE = store_thm ("bir_update_blockB_desc_OK_VARNAME_UNIQUE",
+  ``!env updates up1 up2.
+       bir_update_blockB_desc_OK env updates ==>
+       MEM up1 updates ==>
+       MEM up2 updates ==>
+       (bir_var_name (bir_updateB_desc_var up1) = bir_var_name (bir_updateB_desc_var up2)) ==>
+
+       (up1 = up2)``,
+
+REPEAT GEN_TAC >> REPEAT DISCH_TAC >>
+`?i1. i1 < LENGTH updates /\ (EL i1 updates = up1)` by
+  METIS_TAC[MEM_EL] >>
+`?i2. i2 < LENGTH updates /\ (EL i2 updates = up2)` by
+  METIS_TAC[MEM_EL] >>
+
+MP_TAC (ISPECL [``MAP (\up. bir_var_name (bir_updateB_desc_var up)) updates``, ``i1:num``, ``i2:num``] ALL_DISTINCT_EL_IMP) >>
+FULL_SIMP_TAC list_ss [EL_MAP, bir_update_blockB_desc_OK_def] >>
+STRIP_TAC >>
+FULL_SIMP_TAC std_ss []);
+
+
+
+val bir_update_blockB_desc_TEMP_VAR_NAMES_DIFFERENT = store_thm ("bir_update_blockB_desc_TEMP_VAR_NAMES_DIFFERENT",
+``!var use_temp updates env.
+
+bir_update_blockB_desc_OK env updates /\
+EVERY
+  (\up.
+     bir_var_name (bir_updateB_desc_var up) <>
+     bir_var_name var) updates /\
+~(bir_is_temp_var_name (bir_var_name var)) ==>
+EVERY
+  (\up.
+     bir_var_name (bir_temp_var use_temp var) <>
+     bir_var_name (bir_updateB_desc_temp_var up)) updates``,
+
+SIMP_TAC std_ss [EVERY_MEM, bir_update_blockB_desc_OK_def] >>
+REPEAT GEN_TAC >> STRIP_TAC >>
+REPEAT GEN_TAC >> STRIP_TAC >>
+`bir_updateB_desc_OK env up /\
+ (bir_var_name var <> bir_var_name (bir_updateB_desc_var up))` by METIS_TAC[] >>
+Cases_on `up` >>
+FULL_SIMP_TAC std_ss [bir_updateB_desc_ACCESSORS, bir_temp_var_REWRS,
+  bir_updateB_desc_OK_def] >>
+ASM_SIMP_TAC (std_ss++boolSimps.LIFT_COND_ss) [bir_temp_var_name_11] >>
+METIS_TAC[bir_is_temp_var_name_ALT_DEF]);
+
+
+
+
+val bir_update_blockB_desc_OK_compute_def = Define `
+   bir_update_blockB_desc_OK_compute env (updated_vars : string set) (used_exp_vars : string set) updates =
+   (bir_update_blockB_desc_OK env updates /\
+    EVERY (\up.
+       (bir_var_name (bir_updateB_desc_var up) IN updated_vars) /\
+       (IMAGE bir_var_name (bir_vars_of_exp (bir_updateB_desc_exp up)) SUBSET used_exp_vars))
+      updates)`
+
+val bir_update_blockB_desc_OK_compute_FINAL = store_thm ("bir_update_blockB_desc_OK_compute_FINAL",
+  ``bir_update_blockB_desc_OK_compute env uvs evs updates ==>
+    bir_update_blockB_desc_OK env updates``, SIMP_TAC std_ss [bir_update_blockB_desc_OK_compute_def])
+
+val bir_update_blockB_desc_OK_compute_INIT = store_thm ("bir_update_blockB_desc_OK_compute_INIT",
+  ``!env. bir_update_blockB_desc_OK_compute env {} {} []``,
+SIMP_TAC list_ss [bir_update_blockB_desc_OK_compute_def, bir_update_blockB_desc_OK_NULL]);
+
+val bir_update_blockB_desc_OK_compute_CONS = store_thm ("bir_update_blockB_desc_OK_compute_CONS",
+  ``bir_update_blockB_desc_OK_compute env uvs evs updates ==>
+    bir_updateB_desc_OK env (BUpdateDescB var e v use_temp) ==>
+    ~((bir_var_name var) IN uvs) /\
+    ~((bir_var_name (bir_temp_var use_temp var)) IN evs) ==>
+    bir_update_blockB_desc_OK_compute env ((bir_var_name var) INSERT uvs) (IMAGE bir_var_name (bir_vars_of_exp e) UNION evs) ((BUpdateDescB var e v use_temp)::updates)``,
+
+SIMP_TAC list_ss [bir_update_blockB_desc_OK_compute_def, bir_update_blockB_desc_OK_CONS,
+  bir_updateB_desc_ACCESSORS, IN_INSERT, SUBSET_UNION, IN_IMAGE, SUBSET_DEF,
+  GSYM EVERY_CONJ] >>
+
+SIMP_TAC (std_ss ++ boolSimps.CONJ_ss) [GSYM LEFT_FORALL_IMP_THM, EVERY_MEM,
+  bir_temp_var_REWRS] >>
+METIS_TAC[]);
+
+
+
+(*****************)
+(* Update blocks *)
+(*****************)
+
+val bir_update_blockB_STEP1_def = Define `
+  bir_update_blockB_STEP1 (BUpdateDescB var e v use_temp) =
+  BStmt_Assign (bir_temp_var use_temp var) e`
+
+val bir_update_blockB_STEP2_def = Define `
+  (bir_update_blockB_STEP2 (BUpdateDescB var e v T) =
+     (BStmt_Assign var (BExp_Den (bir_temp_var T var))))
+
+  (* We don't care for case where no temp vars are used *)
+`
+
+val bir_update_blockB_def = Define `bir_update_blockB updates =
+  (MAP bir_update_blockB_STEP1 updates) ++
+  (MAP bir_update_blockB_STEP2 (FILTER bir_updateB_desc_use_temp updates))`
+
+
+(* We will show theorems for the first and the second part of the block
+   separately and then combine them *)
+
+val bir_update_blockB_SEM1 = prove (``!st c l updates.
+
+  (* the initial state is not terminated and the updates are fine in this
+     states environment *)
+  bir_update_blockB_desc_OK st.bst_environ updates /\
+  ~(bir_state_is_terminated st) ==> (?st'.
+
+  (* Then the execution of the first part of the block terminates without
+     running into an error or halting *)
+  (bir_exec_stmtsB (MAP bir_update_blockB_STEP1 updates) (l, c, st) =
+     (REVERSE l, c + LENGTH updates, st')) /\
+  ~(bir_state_is_terminated st') /\
+
+  (* In the resulting state, either the variables in temp themselves or
+     their temp version having been updated to contain now the desired value *)
+  (EVERY (\up.
+        (bir_env_lookup (bir_var_name (bir_updateB_desc_temp_var up)) st'.bst_environ =
+          SOME (bir_var_type (bir_updateB_desc_var up), SOME (bir_updateB_desc_value up)))) updates) /\
+
+  (* All other vars have still the same value *)
+  (!vn. (EVERY (\up. vn <> bir_var_name (bir_updateB_desc_temp_var up)) updates) ==>
+        (bir_env_lookup vn st'.bst_environ = bir_env_lookup vn st.bst_environ)))``,
+
+
+NTAC 3 GEN_TAC >>
+listLib.SNOC_INDUCT_TAC >- (
+  SIMP_TAC list_ss [bir_exec_stmtsB_REWRS]
+) >>
+
+Cases >>
+rename1 `SNOC (BUpdateDescB var e v use_temp) updates` >>
+SIMP_TAC std_ss [bir_update_blockB_desc_OK_SNOC] >>
+REPEAT STRIP_TAC >>
+FULL_SIMP_TAC list_ss [SNOC_APPEND, bir_exec_stmtsB_APPEND, LET_THM, IN_IMAGE,
+  bir_updateB_desc_ACCESSORS, bir_updateB_desc_OK_def] >>
+ASM_SIMP_TAC arith_ss [bir_exec_stmtsB_REWRS, bir_update_blockB_STEP1_def,
+  bir_exec_stmtB_def, LET_THM, OPT_CONS_REWRS, DISJ_IMP_THM, FORALL_AND_THM,
+  bir_updateB_desc_ACCESSORS] >>
+
+
+Cases_on `st.bst_environ` >> rename1 `BEnv env` >>
+Cases_on `st'.bst_environ` >> rename1 `st'.bst_environ = BEnv env'` >>
+
+`EVERY
+  (\up.
+     bir_var_name (bir_temp_var use_temp var) <>
+     bir_var_name (bir_updateB_desc_temp_var up)) updates` by (
+  MATCH_MP_TAC bir_update_blockB_desc_TEMP_VAR_NAMES_DIFFERENT >>
+  Q.EXISTS_TAC `BEnv env` >>
+  ASM_SIMP_TAC std_ss []
+) >>
+
+`?env''. env'' = (env' |+
+                    (if use_temp then
+                         bir_temp_var_name (bir_var_name var)
+                       else bir_var_name var, bir_var_type var,
+                       SOME v))` by METIS_TAC[] >>
+
+
+`bir_exec_stmt_assign (bir_temp_var use_temp var) e st' =
+ (st' with bst_environ := BEnv env'')` by (
+
+  `bir_env_lookup (bir_var_name (bir_temp_var use_temp var)) (BEnv env') =
+   bir_env_lookup (bir_var_name (bir_temp_var use_temp var)) (BEnv env)` by (
+     Q.PAT_X_ASSUM `!vn. _` MATCH_MP_TAC >>
+     ASM_REWRITE_TAC[]
+  ) >>
+
+
+  `bir_env_check_type (bir_temp_var use_temp var) (BEnv env') <=>
+   bir_env_var_is_declared (BEnv env) (bir_temp_var use_temp var)` by (
+    METIS_TAC[bir_env_var_is_declared_def, bir_env_lookup_type_def,
+      bir_env_check_type_def]
+  ) >>
+
+  `bir_eval_exp e (BEnv env') = bir_eval_exp e (BEnv env)` by (
+     MATCH_MP_TAC bir_typing_expTheory.bir_vars_of_exp_THM >>
+     REPEAT STRIP_TAC >>
+     rename1 `var_other IN _` >>
+
+     `bir_env_lookup (bir_var_name var_other) (BEnv env') =
+      bir_env_lookup (bir_var_name var_other) (BEnv env)` by (
+        Q.PAT_X_ASSUM `!vn. _` MATCH_MP_TAC >>
+        FULL_SIMP_TAC std_ss [bir_update_blockB_desc_OK_def, EVERY_MEM] >>
+        METIS_TAC[]
+     ) >>
+     ASM_SIMP_TAC std_ss [bir_env_read_def]
+  ) >>
+
+
+  ASM_SIMP_TAC std_ss [bir_exec_stmt_assign_def,
+    bir_env_write_def, bir_temp_var_REWRS,
+    bir_env_update_def, LET_THM]
+) >>
+
+FULL_SIMP_TAC (std_ss++holBACore_ss) [DISJ_IMP_THM, FORALL_AND_THM,
+  bir_temp_var_REWRS, bir_env_lookup_UPDATE, bir_env_read_UPDATE,
+  bir_state_is_terminated_def, EVERY_MEM]);
+
+
+
+
+
+val bir_update_blockB_SEM2 = prove (``!st c l updates.
+
+(* Now we only update the vars previously stored in a temp value. *)
+let updatesT = FILTER bir_updateB_desc_use_temp updates in
+
+(* We start in a non-terminated state *)
+~(bir_state_is_terminated st) /\
+
+(* All updates are well-formed and the to the temp var has happened before. *)
+(EVERY (\up.
+   ~(bir_is_temp_var_name (bir_var_name (bir_updateB_desc_var up))) /\
+   (type_of_bir_val (bir_updateB_desc_value up) = SOME (bir_var_type (bir_updateB_desc_var up))) /\
+   bir_env_var_is_declared st.bst_environ (bir_updateB_desc_var up) /\
+   (bir_env_lookup (bir_var_name (bir_updateB_desc_temp_var up)) st.bst_environ =
+      SOME (bir_var_type (bir_updateB_desc_var up), SOME (bir_updateB_desc_value up)))) updatesT) /\
+
+(* We don't update anything twice *)
+(ALL_DISTINCT (MAP (\up. bir_var_name (bir_updateB_desc_var up)) updates)) ==> (?st'.
+
+(* Then we terminate successfully ... *)
+(bir_exec_stmtsB (MAP bir_update_blockB_STEP2 updatesT) (l, c, st) = (REVERSE l, c + LENGTH updatesT, st')) /\
+ ~(bir_state_is_terminated st') /\
+
+(* Every update has been performed *)
+EVERY (\up.
+   (bir_env_lookup (bir_var_name (bir_updateB_desc_var up)) st'.bst_environ =
+      SOME (bir_var_type (bir_updateB_desc_var up), SOME (bir_updateB_desc_value up)))) updatesT /\
+
+(* And all other vars remain unchanged *)
+(!vn. (EVERY (\up. vn <> bir_var_name (bir_updateB_desc_var up)) updatesT) ==>
+      (bir_env_lookup vn st'.bst_environ = bir_env_lookup vn st.bst_environ)))``,
+
+
+NTAC 3 GEN_TAC >>
+listLib.SNOC_INDUCT_TAC >- (
+  SIMP_TAC list_ss [bir_exec_stmtsB_REWRS, LET_THM]
+) >>
+
+Cases >>
+rename1 `SNOC (BUpdateDescB var e v use_temp) updates` >>
+Tactical.REVERSE (Cases_on `use_temp`) >> (
+  FULL_SIMP_TAC list_ss [rich_listTheory.FILTER_SNOC, EVERY_SNOC, MAP_SNOC, ALL_DISTINCT_SNOC,
+  DISJ_IMP_THM, FORALL_AND_THM, LET_THM, bir_updateB_desc_ACCESSORS,
+  bir_updateB_desc_OK_def]
+) >>
+REPEAT STRIP_TAC >>
+FULL_SIMP_TAC list_ss [SNOC_APPEND, bir_exec_stmtsB_APPEND, LET_THM] >>
+ASM_SIMP_TAC arith_ss [bir_exec_stmtsB_REWRS, bir_update_blockB_STEP2_def,
+  bir_exec_stmtB_def, LET_THM, OPT_CONS_REWRS, DISJ_IMP_THM, FORALL_AND_THM] >>
+
+Cases_on `st.bst_environ` >> rename1 `BEnv env` >>
+Cases_on `st'.bst_environ` >> rename1 `st'.bst_environ = BEnv env'` >>
+
+
+`bir_env_lookup (bir_temp_var_name (bir_var_name var)) (BEnv env') =
+ bir_env_lookup (bir_temp_var_name (bir_var_name var)) (BEnv env)` by (
+  Q.PAT_X_ASSUM `!vn. _` MATCH_MP_TAC >>
+  FULL_SIMP_TAC list_ss [EVERY_MEM] >>
+  METIS_TAC[bir_is_temp_var_name_ALT_DEF]
+) >>
+
+`!up.
+  MEM up (FILTER bir_updateB_desc_use_temp updates) ==>
+  bir_var_name var <> bir_var_name (bir_updateB_desc_var up)` by (
+  FULL_SIMP_TAC std_ss [MEM_MAP, MEM_FILTER] >>
+  METIS_TAC[]
+) >>
+
+
+`bir_env_lookup (bir_var_name var) (BEnv env') =
+ bir_env_lookup (bir_var_name var) (BEnv env)` by (
+  Q.PAT_X_ASSUM `!vn. _` MATCH_MP_TAC >>
+  FULL_SIMP_TAC std_ss [MEM_MAP, EVERY_MEM] >>
+  METIS_TAC[]
+) >>
+
+`bir_exec_stmt_assign var (BExp_Den (bir_temp_var T var)) st' =
+ (st' with bst_environ := BEnv (env' |+ (bir_var_name var,bir_var_type var,SOME v)))` by (
+
+  FULL_SIMP_TAC std_ss [bir_exec_stmt_assign_def, bir_expTheory.bir_eval_exp_def,
+    bir_env_read_def, bir_temp_var_REWRS, pairTheory.pair_case_thm,
+    LET_THM, bir_env_write_def, bir_env_check_type_def,
+    bir_env_var_is_declared_def, bir_env_lookup_type_def,
+    bir_env_update_def]
+) >>
+
+FULL_SIMP_TAC (std_ss++holBACore_ss) [bir_state_is_terminated_def,
+  bir_env_lookup_UPDATE, EVERY_MEM]);
+
+
+
+
+(* Now combine it! This is what we are really interested in. *)
+val bir_update_blockB_SEM = store_thm ("bir_update_blockB_SEM", ``!st c l updates.
+
+(* We start with valid updates in a non-terminated state. *)
+bir_update_blockB_desc_OK st.bst_environ updates /\
+~(bir_state_is_terminated st) ==>
+
+(* Then we terminate in a state ... *)
+(?st'. (bir_exec_stmtsB (bir_update_blockB updates) (l, c, st) = (REVERSE l, c + LENGTH (bir_update_blockB updates), st')) /\
+  ~(bir_state_is_terminated st') /\
+
+  (* Such that all updates have been performed correctly. *)
+  (EVERY (\up. (bir_env_lookup (bir_var_name (bir_updateB_desc_var up)) st'.bst_environ =
+                   SOME (bir_var_type (bir_updateB_desc_var up), SOME (bir_updateB_desc_value up))) /\
+               (bir_env_lookup (bir_var_name (bir_updateB_desc_temp_var up)) st'.bst_environ =
+                   SOME (bir_var_type (bir_updateB_desc_var up), SOME (bir_updateB_desc_value up))))
+    updates) /\
+
+  (* And nothing else changed *)
+  (!vn. (EVERY (\up. (vn <> bir_var_name (bir_updateB_desc_var up)) /\
+                     (vn <> bir_var_name (bir_updateB_desc_temp_var up))) updates) ==>
+        (bir_env_lookup vn st'.bst_environ = bir_env_lookup vn st.bst_environ)))``,
+
+REPEAT STRIP_TAC >>
+MP_TAC (Q.SPECL [`st`, `c`, `l`, `updates`] bir_update_blockB_SEM1) >>
+ASM_SIMP_TAC std_ss [] >> STRIP_TAC >>
+ASM_SIMP_TAC list_ss [bir_update_blockB_def, bir_exec_stmtsB_APPEND, LET_THM] >>
+
+MP_TAC (Q.SPECL [`st'`, `c+LENGTH (updates:bir_updateB_desc_t list)`,
+  `l`, `updates`] bir_update_blockB_SEM2) >>
+MP_TAC (Q.SPECL [`st.bst_environ`, `updates`] bir_update_blockB_desc_OK_VARNAME_UNIQUE) >>
+ASM_SIMP_TAC std_ss [LET_THM] >> STRIP_TAC >>
+MATCH_MP_TAC (prove (``(A /\ (B ==> C)) ==> ((A ==> B) ==> C)``, PROVE_TAC[])) >>
+STRIP_TAC >- (
+  FULL_SIMP_TAC std_ss [bir_update_blockB_desc_OK_def, bir_temp_var_REWRS, EVERY_MEM,
+    MEM_FILTER] >>
+  GEN_TAC >> STRIP_TAC >>
+  `bir_updateB_desc_OK st.bst_environ up` by METIS_TAC[] >>
+  Cases_on `up` >> rename1 `BUpdateDescB var e v use_temp` >>
+  FULL_SIMP_TAC std_ss [bir_updateB_desc_OK_def, bir_updateB_desc_ACCESSORS] >>
+
+  `bir_env_lookup (bir_var_name var) st'.bst_environ =
+   bir_env_lookup (bir_var_name var) st.bst_environ` suffices_by (
+     FULL_SIMP_TAC std_ss [bir_env_var_is_declared_def, bir_env_lookup_type_def]
+  ) >>
+  Q.PAT_X_ASSUM `!up. _` MATCH_MP_TAC >>
+  Cases >> rename1 `BUpdateDescB var' e' v' use_temp'` >>
+  SIMP_TAC std_ss [bir_updateB_desc_ACCESSORS, bir_temp_var_REWRS] >>
+  Cases_on `use_temp'` >> REWRITE_TAC[] >- (
+    METIS_TAC[bir_is_temp_var_name_ALT_DEF]
+  ) >>
+  METIS_TAC [bir_updateB_desc_var_def, bir_updateB_desc_t_11]
+) >>
+
+STRIP_TAC >>
+FULL_SIMP_TAC list_ss [EVERY_MEM, MEM_FILTER] >>
+Cases >> rename1 `BUpdateDescB var e v use_temp` >>
+STRIP_TAC >> FULL_SIMP_TAC std_ss [bir_updateB_desc_ACCESSORS] >>
+`bir_env_lookup (bir_var_name (bir_temp_var use_temp var)) st''.bst_environ =
+ bir_env_lookup (bir_var_name (bir_temp_var use_temp var)) st'.bst_environ` by (
+
+  Q.PAT_X_ASSUM `!vn. _` MATCH_MP_TAC >>
+  Cases >> rename1 `BUpdateDescB var' e' v' use_temp'` >>
+  SIMP_TAC std_ss [bir_updateB_desc_ACCESSORS, bir_temp_var_REWRS, MEM_FILTER] >>
+  STRIP_TAC >>
+  Cases_on `use_temp` >| [
+    METIS_TAC [bir_update_blockB_desc_OK_def, bir_updateB_desc_OK_def, EVERY_MEM, bir_is_temp_var_name_ALT_DEF],
+    METIS_TAC[bir_updateB_desc_ACCESSORS, bir_updateB_desc_t_11]
+  ]
+) >>
+METIS_TAC[bir_updateB_desc_ACCESSORS, bir_temp_var_REWRS]);
+
+
+val _ = export_theory();
